updates

Veritas.BinTreePtr.fst
@@ -5,6 +5,130 @@ open Veritas.BinTree
 (* pointer based descendant relation *)
 noeq type pdesc: ptrfn -> bin_tree_node -> bin_tree_node -> Type = 
   | PSelf: pf: ptrfn -> n:bin_tree_node -> pdesc pf n n
-  | PTran: pf: ptrfn -> d:bin_tree_node -> a:bin_tree_node -> _:(pdesc pf d a) -> 
-           c:bin_tree_dir{Some? (pf d c)} ->
-           pdesc pf (Some?.v (pf d c)) a
+  | PTran: pf: ptrfn -> d:bin_tree_node -> d':bin_tree_node -> _:(pdesc pf d d') -> 
+           a:bin_tree_node ->
+           c:bin_tree_dir{Some? (pf a c) /\ Some?.v (pf a c) = d'} ->
+           pdesc pf d a
+
+let rec is_pdesc_aux 
+  (pf: ptrfn) 
+  (d:bin_tree_node) 
+  (a:bin_tree_node{is_proper_desc d a /\ depth d > depth a}): Tot bool
+  (decreases (depth d - depth a)) = 
+  let c = desc_dir d a in
+  match pf a c with
+  | None -> false
+  | Some d' -> if d' = d then true
+               else if is_desc d d' then (
+                 lemma_desc_depth_monotonic d' (child c a);
+                 lemma_proper_desc_depth_monotonic d d';
+                 is_pdesc_aux pf d d'
+               )
+               else
+                 false
+                 
+let is_pdesc (pf:ptrfn) (d a: bin_tree_node): Tot bool = 
+  if d = a then true
+  else if is_desc d a then (
+    lemma_proper_desc_depth_monotonic d a;
+    is_pdesc_aux pf d a
+  )
+  else false
+
+let rec lemma_pdesc_implies_desc_t (pf: ptrfn) (d a: bin_tree_node) (prf: pdesc pf d a):
+  Lemma (requires (True))
+        (ensures (is_desc d a))
+        (decreases prf) = 
+  match prf with
+  | PSelf pf' n' -> lemma_desc_reflexive n'
+  | PTran pf' d1 d' prf' a1 c -> 
+    lemma_pdesc_implies_desc_t pf d d' prf';
+    lemma_parent_ancestor (child c a);
+    lemma_proper_desc_transitive2 d' (child c a) a;
+    lemma_desc_transitive d d' a
+
+let rec lemma_pdesc_correct (pf:ptrfn) (d a: bin_tree_node) (prf: pdesc pf d a):
+  Lemma (requires (True))
+        (ensures (is_pdesc pf d a = true))
+        (decreases prf) = 
+  match prf with
+  | PSelf _ _  -> ()
+  | PTran _  _ d' prf' _ c -> 
+
+    lemma_pdesc_implies_desc_t pf d d' prf';
+    assert(is_desc d d');
+
+    lemma_pdesc_correct pf d d' prf';
+    assert(is_pdesc pf d d');
+
+    lemma_parent_ancestor (child c a);
+    lemma_proper_desc_transitive2 d' (child c a) a;
+    lemma_desc_transitive d d' a;
+    assert(is_desc d a);
+
+    if d = a then ()
+    else (
+      lemma_proper_desc_depth_monotonic d a;
+      lemma_desc_transitive d d' (child c a);
+      assert(desc_dir d a = c);
+
+      if d' = d then ()
+      else ()
+    )
+
+let rec lemma_pdesc_correct2_aux 
+  (pf:ptrfn) 
+  (d:bin_tree_node) 
+  (a:bin_tree_node{is_pdesc pf d a /\ depth d >= depth a}): 
+  Tot (pdesc pf d a) 
+  (decreases (depth d - depth a)) = 
+  if d = a then PSelf pf d
+  else (
+    lemma_proper_desc_depth_monotonic d a;
+    let c = desc_dir d a in    
+    let d' = Some?.v (pf a c) in
+    if d' = d then PTran pf d d (PSelf pf d) a c
+    else (
+      lemma_desc_depth_monotonic d' (child c a);
+      lemma_proper_desc_depth_monotonic d d';
+      let prfdd' = lemma_pdesc_correct2_aux pf d d' in
+      PTran pf d d' prfdd' a c
+    )
+  )
+
+let lemma_pdesc_implies_desc 
+  (pf:ptrfn) 
+  (d: bin_tree_node)
+  (a: bin_tree_node{is_pdesc pf d a}):
+  Lemma (requires (True))
+        (ensures (is_desc d a)) = 
+  if d = a then lemma_desc_reflexive d
+  else ()
+
+let lemma_pdesc_correct2
+  (pf:ptrfn) 
+  (d:bin_tree_node) 
+  (a:bin_tree_node{is_pdesc pf d a}): Tot (pdesc pf d a) =
+  lemma_pdesc_implies_desc pf d a;
+  lemma_desc_depth_monotonic d a;
+  lemma_pdesc_correct2_aux pf d a
+
+let lemma_pdesc_reflexive (pf: ptrfn) (a: bin_tree_node):
+  Lemma (is_pdesc pf a a) = ()
+
+let rec lemma_pdesc_transitive_t (pf: ptrfn) (n1 n2 n3: bin_tree_node) 
+  (prf12: pdesc pf n1 n2) (prf23: pdesc pf n2 n3): Tot (pdesc pf n1 n3) (decreases prf23) = 
+  match prf23 with
+  | PSelf pf _ -> prf12
+  | PTran pf _ n' prf2' _ c' -> 
+    let prf1' = lemma_pdesc_transitive_t pf n1 n2 n' prf12 prf2' in
+    PTran pf n1 n' prf1' n3 c'
+
+let lemma_pdesc_transitive (pf: ptrfn) (a b c: bin_tree_node):
+  Lemma (requires (is_pdesc pf a b /\ is_pdesc pf b c))
+        (ensures (is_pdesc pf a c)) = 
+  let prf_ab = lemma_pdesc_correct2 pf a b in
+  let prf_bc = lemma_pdesc_correct2 pf b c in
+  let prf_ac = lemma_pdesc_transitive_t pf a b c prf_ab prf_bc in
+  lemma_pdesc_correct pf a c prf_ac
+
